Using record instead of dtuple3 for BIT_STRING.

src/asn1/ASN1.Spec.Value.BIT_STRING.fst
@@ -79,11 +79,12 @@ let synth_asn1_bit_string
   (l: asn1_value_length_of_type BIT_STRING)
   (raw: parse_filter_refine (filter_asn1_bit_string l))
 : GTot (value: datatype_of_asn1_type BIT_STRING {
-               let (|len, unused_bits, s|) = value in
-               l == v len })
+               l == v value.len })
 = let unused_bits: n: asn1_int32 {0 <= v n /\ v n <= 7} = cast raw.[0] in
   let s32 = B32.hide (Seq.slice raw 1 l) in
-  (|u l, unused_bits, s32|)
+  { len         = u l;
+    unused_bits = unused_bits;
+    s           = s32 }
 
 /// Prove our decode function is injective
 #push-options "--z3rlimit 16"
@@ -114,13 +115,11 @@ noextract
 let synth_asn1_bit_string_inverse
   (l: asn1_value_length_of_type BIT_STRING)
   (value: datatype_of_asn1_type BIT_STRING {
-          let (|len, unused_bits, s|) = value in
-          l == v len })
+          l == v value.len })
 : GTot (raw: parse_filter_refine (filter_asn1_bit_string l) { value == synth_asn1_bit_string l raw })
-= let (|len, unused_bits, s32|) = value in
-  let raw = cast unused_bits `Seq.cons` B32.reveal s32 in
-  let (|len', unused_bits', s32'|) = synth_asn1_bit_string l raw in
-  B32.extensionality s32 s32';
+= let raw = cast value.unused_bits `Seq.cons` B32.reveal value.s in
+  let value' = synth_asn1_bit_string l raw in
+  B32.extensionality value.s value'.s;
   raw
 
 noextract
@@ -134,8 +133,7 @@ let parse_asn1_bit_string
   (l: asn1_value_length_of_type BIT_STRING)
 : parser (parse_asn1_bit_string_kind l)
          (value: datatype_of_asn1_type BIT_STRING {
-                 let (|len, unused_bits, s|) = value in
-                 l == v len })
+                 l == v value.len })
 = synth_asn1_bit_string_injective l;
   parse_seq_flbytes l
   `parse_filter`
@@ -199,8 +197,7 @@ noextract
 let serialize_asn1_bit_string_unfold
   (l: asn1_value_length_of_type BIT_STRING)
   (value: datatype_of_asn1_type BIT_STRING {
-                 let (|len, unused_bits, s|) = value in
-                 l == v len })
+                 l == v value.len })
 : Lemma (
   serialize (serialize_asn1_bit_string l) value ==
   serialize (serialize_seq_flbytes l) (synth_asn1_bit_string_inverse l value))
@@ -221,8 +218,7 @@ noextract
 let serialize_asn1_bit_string_size
   (l: asn1_value_length_of_type BIT_STRING)
   (value: datatype_of_asn1_type BIT_STRING {
-                 let (|len, unused_bits, s|) = value in
-                 l == v len })
+                 l == v value.len })
 : Lemma (
   Seq.length (serialize (serialize_asn1_bit_string l) value) == l)
 = parser_kind_prop_equiv (parse_asn1_bit_string_kind l) (parse_asn1_bit_string l);
@@ -237,8 +233,7 @@ noextract
 let parser_tag_of_bit_string
   (x: datatype_of_asn1_type BIT_STRING)
 : GTot (the_asn1_type BIT_STRING & asn1_value_int32_of_type BIT_STRING)
-= let (|len, unused_bits, s32|) = x in
-  (BIT_STRING, len)
+= (BIT_STRING, x.len)
 
 ///
 /// A pair of aux parser/serializer, which explicitly coerce the `BIT_STRING` value
@@ -256,8 +251,7 @@ noextract
 let synth_asn1_bit_string_V
   (tag: (the_asn1_type BIT_STRING & asn1_value_int32_of_type BIT_STRING))
   (value: datatype_of_asn1_type BIT_STRING {
-                 let (|len, unused_bits, s|) = value in
-                 v (snd tag) == v len })
+                 v (snd tag) == v value.len })
 : GTot (refine_with_tag parser_tag_of_bit_string tag)
 = value
 
@@ -269,8 +263,7 @@ let synth_asn1_bit_string_V_inverse
   (tag: (the_asn1_type BIT_STRING & asn1_value_int32_of_type BIT_STRING))
   (value': refine_with_tag parser_tag_of_bit_string tag)
 : GTot (value: datatype_of_asn1_type BIT_STRING {
-                 let (|len, unused_bits, s|) = value in
-                 v (snd tag) == v len /\
+                 v (snd tag) == v value.len /\
                  value' == synth_asn1_bit_string_V tag value })
 = value'
 
@@ -443,13 +436,12 @@ noextract
 let serialize_asn1_bit_string_TLV_unfold
   (value: datatype_of_asn1_type BIT_STRING)
 : Lemma (
-  let (|len, unused_bits, s32|) = value in
   serialize serialize_asn1_bit_string_TLV value ==
   serialize (serialize_asn1_tag_of_type BIT_STRING) BIT_STRING
   `Seq.append`
-  serialize (serialize_asn1_length_of_type BIT_STRING) len
+  serialize (serialize_asn1_length_of_type BIT_STRING) value.len
   `Seq.append`
-  serialize (serialize_asn1_bit_string (v len)) value
+  serialize (serialize_asn1_bit_string (v value.len)) value
 )
 = serialize_nondep_then_eq
   (* s1 *) (serialize_asn1_tag_of_type BIT_STRING)
@@ -471,13 +463,11 @@ noextract
 let serialize_asn1_bit_string_TLV_size
   (value: datatype_of_asn1_type BIT_STRING)
 : Lemma (
-  let (|len, unused_bits, s32|) = value in
   Seq.length (serialize serialize_asn1_bit_string_TLV value) ==
-  1 + length_of_asn1_length len + v len)
-= let (|len, unused_bits, s32|) = value in
-  serialize_asn1_bit_string_TLV_unfold value;
+  1 + length_of_asn1_length value.len + v value.len)
+= serialize_asn1_bit_string_TLV_unfold value;
   serialize_asn1_tag_of_type_size BIT_STRING BIT_STRING;
-  serialize_asn1_length_size len;
-  serialize_asn1_length_of_type_eq BIT_STRING len;
-  serialize_asn1_bit_string_size (v len) value
+  serialize_asn1_length_size value.len;
+  serialize_asn1_length_of_type_eq BIT_STRING value.len;
+  serialize_asn1_bit_string_size (v value.len) value
 #pop-options
